inductive_proof/Observed-remove_set/App_comm.fst
@@ -1,7 +1,5 @@
 module App_comm
 
-open FStar.Seq
-open FStar.Ghost
 module S = Set_extended
 
 #set-options "--query_stats"
@@ -11,7 +9,6 @@ type concrete_st = S.set (nat * nat)
 let init_st = S.empty
 
 let eq (a b:concrete_st) =
-  //a == b
   S.equal a b
 
 // few properties of equivalence relation
@@ -51,20 +48,16 @@ let lem_do (a b:concrete_st) (op:op_t)
            (ensures eq (do a op) (do b op)) = ()
 
 //conflict resolution
-let resolve_conflict (x:op_t) (y:op_t{fst x <> fst y}) : (l:log{(forall e. mem e l <==> (e == x \/ e == y))}) =
-  if (get_ele x = get_ele y && Add? (snd x) && Rem? (snd y)) then 
-    cons y (cons x empty) else
-      cons x (cons y empty)
+let resolve_conflict (x:op_t) (y:op_t{fst x <> fst y}) : resolve_conflict_res =
+  if get_ele x = get_ele y && Add? (snd x) && Rem? (snd y) then First else Second
 
 let resolve_conflict_prop (x y:op_t) 
   : Lemma (requires fst x <> fst y)
-          (ensures Seq.length (resolve_conflict x y) = 2 /\
-                   (last (resolve_conflict x y) = x <==> (Add? (snd x) /\ Rem? (snd y) /\ get_ele x = get_ele y)) /\
-                   (last (resolve_conflict x y) <> x <==> last (resolve_conflict x y) = y) /\
-                   (last (resolve_conflict x y) = y <==> ((Add? (snd x) /\ Rem? (snd y) /\ get_ele x <> get_ele y) \/
-                                                        (Add? (snd x) /\ Add? (snd y)) \/
-                                                        (Rem? (snd x) /\ Rem? (snd y)) \/
-                                                        (Rem? (snd x) /\ Add? (snd y)))))
+          (ensures (First? (resolve_conflict x y) <==> (Add? (snd x) /\ Rem? (snd y) /\ get_ele x = get_ele y)) /\
+                   (Second? (resolve_conflict x y) <==> ((Add? (snd x) /\ Rem? (snd y) /\ get_ele x <> get_ele y) \/
+                                                       (Add? (snd x) /\ Add? (snd y)) \/
+                                                       (Rem? (snd x) /\ Rem? (snd y)) \/
+                                                       (Rem? (snd x) /\ Add? (snd y)))))
   = ()
 
 (*merge l a b == (intersect l a b) U (a - l) U (b - l)*)
@@ -162,7 +155,7 @@ let lem_lca_eq''_base_pre (lca s1 s2:st) (last1 last2:op_t)
 let lem_l2a_l1r_eq''_base_ind (lca s1 s2:st) (last1 last2:op_t)
   : Lemma (requires length (ops_of lca) > 0 /\
                     ops_of s1 = ops_of lca /\ ops_of s2 = ops_of lca /\
-                    Add? (snd last2) /\ //Rem? (snd last1) /\ get_ele last1 = get_ele last2 /\
+                    Add? (snd last2) /\ 
                     not (mem_id (fst last1) (ops_of lca)) /\
                     not (mem_id (fst last2) (ops_of lca)) /\
 
@@ -183,7 +176,7 @@ let lem_l2a_l1r_eq''_base_ind (lca s1 s2:st) (last1 last2:op_t)
 
 let rec lem_l2a_l1r_eq''_base (lca s1 s2:st) (last1 last2:op_t)
   : Lemma (requires ops_of s1 = ops_of lca /\ ops_of s2 = ops_of lca /\
-                    Add? (snd last2) /\ //Rem? (snd last1) /\ get_ele last1 = get_ele last2 /\ 
+                    Add? (snd last2) /\ 
                     not (mem_id (fst last1) (ops_of lca)) /\
                     not (mem_id (fst last2) (ops_of lca)))
           (ensures eq (do (concrete_merge (v_of lca) (do (v_of s1) last1) (v_of s2)) last2)
@@ -201,7 +194,7 @@ let rec lem_l2a_l1r_eq''_base (lca s1 s2:st) (last1 last2:op_t)
 let lem_l2a_l1r_eq''_s10_s2_gt0 (lca s1 s2:st) (last1 last2:op_t)
   : Lemma (requires ops_of s1 = ops_of lca /\
                     length (ops_of s2) > length (ops_of lca) /\
-                    Add? (snd last2) /\ //Rem? (snd last1) /\ get_ele last1 = get_ele last2 /\
+                    Add? (snd last2) /\ 
                     (let s2' = inverse_st s2 in
                     
                      eq (do (concrete_merge (v_of lca) (do (v_of s1) last1) (v_of s2')) last2)
@@ -596,10 +589,10 @@ let not_add_eq (lca s1 s2:st)
   assert ((Add? (snd last1) /\ get_ele last1 = get_ele last2) ==> not (commutative last1 last2));
   resolve_conflict_prop last2 last1;
   assert ((Add? (snd last1) /\ get_ele last1 = get_ele last2) ==> 
-                last (resolve_conflict last2 last1) = last1);
+                First? (resolve_conflict last2 last1));
   assert ((Add? (snd last1) /\ get_ele last1 = get_ele last2) ==> 
                 not (commutative last2 last1) /\
-                last (resolve_conflict last2 last1) = last1 /\
+                First? (resolve_conflict last2 last1) /\
                 commutative_seq last1 suf);
   assert ((Add? (snd last1) /\ get_ele last1 = get_ele last2) ==> exists_triple last2 (diff (ops_of s1) (ops_of lca)));
   assert (~ (Add? (snd last1) /\ get_ele last1 = get_ele last2)); ()
@@ -788,7 +781,7 @@ let lem_l2r (lca s1 s2:st)
                      Rem? (snd last2) /\
                      not (exists_triple last1 (diff (ops_of s2) (ops_of lca))) /\
                      not (exists_triple last2 (diff (ops_of s1) (ops_of lca))) /\
-                     last (resolve_conflict last1 last2) = last2 /\
+                     Second? (resolve_conflict last1 last2) /\
                      is_prefix (ops_of lca) (ops_of (inverse_st s2))))
           (ensures (let _, last2 = un_snoc (ops_of s2) in
                     eq (do (concrete_merge (v_of lca) (v_of s1) (v_of (inverse_st s2))) last2)
@@ -1026,19 +1019,20 @@ let lem_exists (lastop:op_t) (l:log)
                     (forall r. mem r suf /\ get_ele r = get_ele lastop ==> Add? (snd r))))))
   = ()
 
-let linearizable_gt0_s1'_op (lca s1 s2:st)
+let linearizable_gt0_s2'_op (lca s1 s2:st)
   : Lemma (requires common_pre lca s1 s2 /\ 
                     (let _, last1 = un_snoc (ops_of s1) in
                      let _, last2 = un_snoc (ops_of s2) in
                      fst last1 <> fst last2 /\
-                     exists_triple last1 (diff (ops_of s2) (ops_of lca)) /\
+                     exists_triple last1 (diff (ops_of s2) (ops_of lca)) /\                   
                      (let (_, op2, suf2) = find_triple last1 (diff (ops_of s2) (ops_of lca)) in
-                      suf2 = snd (pre_suf (ops_of s2) op2))))
+                     suf2 == snd (pre_suf (ops_of s2) op2))))
+     
           (ensures (let _, last1 = un_snoc (ops_of s1) in
                     let (pre2, op2, suf2) = find_triple last1 (diff (ops_of s2) (ops_of lca)) in
-                    let s2' = inverse_st_op s2 op2 in
-                       eq (do (concrete_merge (v_of lca) (v_of s1) (v_of s2')) op2)
-                          (concrete_merge (v_of lca) (v_of s1) (do (v_of s2') op2)))) =
+                    let s2' = inverse_st_op s2 op2 in                      
+                    eq (do (concrete_merge (v_of lca) (v_of s1) (v_of s2')) op2)
+                       (concrete_merge (v_of lca) (v_of s1) (do (v_of s2') op2)))) =
   let _, last1 = un_snoc (ops_of s1) in
   let pre2, op2, suf2 = find_triple last1 (diff (ops_of s2) (ops_of lca)) in
   let s2' = inverse_st_op s2 op2 in
@@ -1050,20 +1044,21 @@ let linearizable_gt0_s1'_op (lca s1 s2:st)
   lem_suf_equal2 (ops_of lca) (ops_of s2) op2;
   lem_inverse_op (ops_of lca) (ops_of s2) op2;
   lem_l2a_l1r_eq'' lca (inverse_st s1) s2' last1 op2
-
-let linearizable_gt0_s2'_op (lca s1 s2:st)
+  
+let linearizable_gt0_s1'_op (lca s1 s2:st)
   : Lemma (requires common_pre lca s1 s2 /\ 
                     (let _, last1 = un_snoc (ops_of s1) in
                      let _, last2 = un_snoc (ops_of s2) in
-                     fst last1 <> fst last2 /\
+                     fst last1 <> fst last2 /\                                          
                      not (exists_triple last1 (diff (ops_of s2) (ops_of lca))) /\
-                     exists_triple last2 (diff (ops_of s1) (ops_of lca)) /\
+                     exists_triple last2 (diff (ops_of s1) (ops_of lca)) /\                    
                      (let (_, op1, suf1) = find_triple last2 (diff (ops_of s1) (ops_of lca)) in
-                      suf1 = snd (pre_suf (ops_of s1) op1))))
+                     suf1 == snd (pre_suf (ops_of s1) op1))))
+     
           (ensures (let _, last2 = un_snoc (ops_of s2) in
                     let (pre1, op1, suf2) = find_triple last2 (diff (ops_of s1) (ops_of lca)) in
-                    let s1' = inverse_st_op s1 op1 in
-                       eq (do (concrete_merge (v_of lca) (v_of s1') (v_of s2)) op1)
+                    let s1' = inverse_st_op s1 op1 in                     
+                     eq (do (concrete_merge (v_of lca) (v_of s1') (v_of s2)) op1)
                           (concrete_merge (v_of lca) (do (v_of s1') op1) (v_of s2)))) =
   let _, last2 = un_snoc (ops_of s2) in
   let pre1, op1, suf1 = find_triple last2 (diff (ops_of s1) (ops_of lca)) in
@@ -1107,10 +1102,10 @@ let rem_add_lastop_neq_ele (lca s1 s2:st)
   
   assert (Rem? (snd last2) /\ get_ele last1 = get_ele last2 ==> commutative_seq last1 suf); 
   assert (Rem? (snd last2) /\ get_ele last1 = get_ele last2 ==> not (commutative last1 last2));
-  assert (Rem? (snd last2) /\ get_ele last1 = get_ele last2 ==> last (resolve_conflict last1 last2) = last1);
+  assert (Rem? (snd last2) /\ get_ele last1 = get_ele last2 ==> First? (resolve_conflict last1 last2));
   assert (Rem? (snd last2) /\ get_ele last1 = get_ele last2 ==> 
           (not (commutative last1 last2) /\
-          last (resolve_conflict last1 last2) = last1 /\
+          First? (resolve_conflict last1 last2) /\
           commutative_seq last1 suf));
   assert (Rem? (snd last2) /\ get_ele last1 = get_ele last2 ==> 
            exists_triple last2 (diff (ops_of s1) (ops_of lca)));
@@ -1123,7 +1118,7 @@ let linearizable_gt0_s1' (lca s1 s2:st)
                      fst last1 <> fst last2 /\
                      not (exists_triple last1 (diff (ops_of s2) (ops_of lca))) /\
                      not (exists_triple last2 (diff (ops_of s1) (ops_of lca))) /\
-                     last (resolve_conflict last1 last2) = last1 /\
+                     First? (resolve_conflict last1 last2) /\
                      is_prefix (ops_of lca) (ops_of (inverse_st s1))))
           (ensures (let _, last1 = un_snoc (ops_of s1) in
                     eq (do (concrete_merge (v_of lca) (v_of (inverse_st s1)) (v_of s2)) last1)
@@ -1146,15 +1141,12 @@ let linearizable_gt0_s2' (lca s1 s2:st)
                      fst last1 <> fst last2 /\
                      not (exists_triple last1 (diff (ops_of s2) (ops_of lca))) /\
                      not (exists_triple last2 (diff (ops_of s1) (ops_of lca))) /\
-                     last (resolve_conflict last1 last2) <> last1 /\
+                     Second? (resolve_conflict last1 last2) /\
                      is_prefix (ops_of lca) (ops_of (inverse_st s2))))
           (ensures (let _, last2 = un_snoc (ops_of s2) in
                     eq (do (concrete_merge (v_of lca) (v_of s1) (v_of (inverse_st s2))) last2)
                        (concrete_merge (v_of lca) (v_of s1) (v_of s2)))) = 
-  let _, last1 = un_snoc (ops_of s1) in
   let _, last2 = un_snoc (ops_of s2) in
-  resolve_conflict_prop last1 last2;
-  assert (last (resolve_conflict last1 last2) = last2);
   if Add? (snd last2) then
     lem_l2a lca s1 s2
   else lem_l2r lca s1 s2
